matrix prog

proofs/fstar/extraction-edited/Libcrux.Kem.Kyber.Matrix.fst
@@ -126,68 +126,61 @@ let compute_As_plus_e v_K matrix_A s_as_ntt error_as_ntt =
   result  
 #pop-options 
 
+#push-options "--ifuel 0 --z3rlimit 100"
 let compute_message #p v_K m_v secret_as_ntt u_as_ntt = 
-  let result:Libcrux.Kem.Kyber.Arithmetic.wfPolynomialRingElement =
+  let result:Libcrux.Kem.Kyber.Arithmetic.t_PolynomialRingElement_b (v v_K * 3328) =
     Libcrux.Kem.Kyber.Arithmetic.cast_poly_b Libcrux.Kem.Kyber.Arithmetic.impl__PolynomialRingElement__ZERO
   in
-  let acc_t = Libcrux.Kem.Kyber.Arithmetic.wfPolynomialRingElement in
+  let acc_t = Libcrux.Kem.Kyber.Arithmetic.t_PolynomialRingElement_b (v v_K * 3328) in
   [@ inline_let]
-  let inv = fun (acc:acc_t) (i:usize) -> True in
-  let result:Libcrux.Kem.Kyber.Arithmetic.wfPolynomialRingElement =
+  let inv = fun (acc:acc_t) (i:usize) -> 
+             (v i <= v v_K) /\
+             (poly_range #(v v_K * 3328) acc (v i * 3328))
+  in
+  let result:Libcrux.Kem.Kyber.Arithmetic.t_PolynomialRingElement_b (v v_K * 3328) =
     Rust_primitives.Iterators.foldi_range #_ #acc_t #inv {
               Core.Ops.Range.f_start = sz 0;
               Core.Ops.Range.f_end = v_K
             }
       result 
       (fun result i ->
-          let result:Libcrux.Kem.Kyber.Arithmetic.wfPolynomialRingElement = result in
           let i:usize = i in
+          let result:t_PolynomialRingElement_b (v i * 3328) = 
+            down_cast_poly_b #(v v_K * 3328) #(v i * 3328) result in
           let product:Libcrux.Kem.Kyber.Arithmetic.wfPolynomialRingElement =
             Libcrux.Kem.Kyber.Ntt.ntt_multiply (secret_as_ntt.[ i ]
                 <:
                 Libcrux.Kem.Kyber.Arithmetic.wfPolynomialRingElement)
               (u_as_ntt.[ i ] <: Libcrux.Kem.Kyber.Arithmetic.wfPolynomialRingElement)
           in
-          admit(); //pre for add_to_ring
-          let result:Libcrux.Kem.Kyber.Arithmetic.wfPolynomialRingElement =
+          let result:Libcrux.Kem.Kyber.Arithmetic.t_PolynomialRingElement_b ((v i+1) * 3328)  =
             Libcrux.Kem.Kyber.Arithmetic.add_to_ring_element v_K result product
           in
+          let result = cast_poly_b #((v i + 1) * 3328) #(v v_K * 3328) result in
+          assert(inv result (i +! sz 1));
           result)
   in
-  admit();
-  let result:Libcrux.Kem.Kyber.Arithmetic.t_PolynomialRingElement_b (128*v v_K*3328) =
-    Libcrux.Kem.Kyber.Ntt.invert_ntt_montgomery v_K result
+  let acc_t = t_PolynomialRingElement_b (64*v v_K*3328) in
+  let result:acc_t = Libcrux.Kem.Kyber.Ntt.invert_ntt_montgomery v_K result
   in
-  let acc_t = Libcrux.Kem.Kyber.Arithmetic.wfPolynomialRingElement in
   [@ inline_let]
-  let inv = fun (acc:acc_t) (i:usize) -> True in
-  let result:Libcrux.Kem.Kyber.Arithmetic.wfPolynomialRingElement =
-    Rust_primitives.Iterators.foldi_range #_ #acc_t #inv {
+  let inv = fun (acc:acc_t) (i:usize) ->
+    (v i <= 256) /\
+    (forall (j:usize). (v j < v i) ==> i32_range ((acc <: t_PolynomialRingElement_b (64* v v_K * 3328)).f_coefficients.[j]) 3328) in
+  let result:Libcrux.Kem.Kyber.Arithmetic.t_PolynomialRingElement_b (64*v v_K*3328) =
+    Rust_primitives.Iterators.foldi_range #_ #_ #inv {
               Core.Ops.Range.f_start = sz 0;
               Core.Ops.Range.f_end = Libcrux.Kem.Kyber.Constants.v_COEFFICIENTS_IN_RING_ELEMENT
             }
       result 
       (fun result i ->
-          let result:Libcrux.Kem.Kyber.Arithmetic.wfPolynomialRingElement = result in
           let i:usize = i in
-          assume (range (v #i32_inttype result.Libcrux.Kem.Kyber.Arithmetic.f_coefficients.[i] *  1441) i32_inttype);
-          let coefficient_normal_form = 
+          let coefficient_normal_form: i32_b (nat_div_ceil (306921472*v v_K) 65536 + 1665) = 
               Libcrux.Kem.Kyber.Arithmetic.montgomery_reduce 
-                           (Libcrux.Kem.Kyber.Arithmetic.mul_i32_b #3328 #1441
+                           (Libcrux.Kem.Kyber.Arithmetic.mul_i32_b #(64 * v v_K * 3328) #1441
                            result.Libcrux.Kem.Kyber.Arithmetic.f_coefficients.[ i ] 
                            (1441l <: Libcrux.Kem.Kyber.Arithmetic.i32_b 1441)) in
-          assume (range (v #i32_inttype m_v.Libcrux.Kem.Kyber.Arithmetic.f_coefficients.[i] - v coefficient_normal_form) i32_inttype);
-//          assume (Libcrux.Kem.Kyber.Arithmetic.barrett_pre (m_v.(i) -! coefficient_normal_form));
-
-          let result:Libcrux.Kem.Kyber.Arithmetic.wfPolynomialRingElement =
-            {
-              result with
-              Libcrux.Kem.Kyber.Arithmetic.f_coefficients
-              =
-              Rust_primitives.Hax.Monomorphized_update_at.update_at_usize result
-                  .Libcrux.Kem.Kyber.Arithmetic.f_coefficients
-                i
-                (Libcrux.Kem.Kyber.Arithmetic.barrett_reduce ((m_v
+          let resulti : i32_b 3328 = (Libcrux.Kem.Kyber.Arithmetic.barrett_reduce ((m_v
                           .Libcrux.Kem.Kyber.Arithmetic.f_coefficients.[ i ]
                         <:
                         i32) -!
@@ -195,86 +188,77 @@ let compute_message #p v_K m_v secret_as_ntt u_as_ntt =
                       <:
                       i32)
                   <:
-                  i32)
-            }
-            <:
-            Libcrux.Kem.Kyber.Arithmetic.wfPolynomialRingElement
-          in
-          result)
-  in
-  admit(); //P-F
-  result
-
-// TODO: error_2_ changed from `t_PolynomialRingElement_b 3` to `t_PolynomialRingElement_b 7`
-let compute_ring_element_v v_K tt_as_ntt r_as_ntt error_2_ message =
-  let result:Libcrux.Kem.Kyber.Arithmetic.wfPolynomialRingElement =
-    Libcrux.Kem.Kyber.Arithmetic.cast_poly_b Libcrux.Kem.Kyber.Arithmetic.impl__PolynomialRingElement__ZERO
-  in
-  let result:Libcrux.Kem.Kyber.Arithmetic.wfPolynomialRingElement =
-    Core.Iter.Traits.Iterator.f_fold (Core.Iter.Traits.Collect.f_into_iter ({
-              Core.Ops.Range.f_start = sz 0;
-              Core.Ops.Range.f_end = v_K
-            }
-            <:
-            Core.Ops.Range.t_Range usize)
-        <:
-        Core.Ops.Range.t_Range usize)
-      result
-      (fun result i ->
-          let result:Libcrux.Kem.Kyber.Arithmetic.wfPolynomialRingElement = result in
-          let i:usize = i in
-          admit();
-          let product:Libcrux.Kem.Kyber.Arithmetic.wfPolynomialRingElement =
-            Libcrux.Kem.Kyber.Ntt.ntt_multiply (tt_as_ntt.[ i ]
-                <:
-                Libcrux.Kem.Kyber.Arithmetic.wfPolynomialRingElement)
-              (r_as_ntt.[ i ] <: Libcrux.Kem.Kyber.Arithmetic.wfPolynomialRingElement)
-          in
-          admit(); //pre for add_to_ring_element
-          let result:Libcrux.Kem.Kyber.Arithmetic.wfPolynomialRingElement =
-            Libcrux.Kem.Kyber.Arithmetic.add_to_ring_element v_K result product
-          in
-          result)
-  in
-  admit();
-  let result:Libcrux.Kem.Kyber.Arithmetic.wfPolynomialRingElement =
-    Libcrux.Kem.Kyber.Ntt.invert_ntt_montgomery v_K result
-  in
-  let result:Libcrux.Kem.Kyber.Arithmetic.wfPolynomialRingElement =
-    Core.Iter.Traits.Iterator.f_fold (Core.Iter.Traits.Collect.f_into_iter ({
-              Core.Ops.Range.f_start = sz 0;
-              Core.Ops.Range.f_end = Libcrux.Kem.Kyber.Constants.v_COEFFICIENTS_IN_RING_ELEMENT
-            }
-            <:
-            Core.Ops.Range.t_Range usize)
-        <:
-        Core.Ops.Range.t_Range usize)
-      result
-      (fun result i ->
-          let result:Libcrux.Kem.Kyber.Arithmetic.wfPolynomialRingElement = result in
-          let i:usize = i in
-          assume (range (v #i32_inttype result.Libcrux.Kem.Kyber.Arithmetic.f_coefficients.[i] * 1441) i32_inttype);
-          let coefficient_normal_form =
-            Libcrux.Kem.Kyber.Arithmetic.montgomery_reduce 
-                    (Libcrux.Kem.Kyber.Arithmetic.mul_i32_b #3328 #1441
-                    (result.Libcrux.Kem.Kyber.Arithmetic.f_coefficients.[ i ])
-                    (1441l <: Libcrux.Kem.Kyber.Arithmetic.i32_b 1441))
-          in
-          assume (range (v coefficient_normal_form +
-                        v #i32_inttype error_2_.f_coefficients.[ i ]) i32_inttype);
-          assume (range (v coefficient_normal_form +
-                        v #i32_inttype error_2_.f_coefficients.[ i ] +
-                        v #i32_inttype message.f_coefficients.[ i ]) i32_inttype);
-//          assume (Libcrux.Kem.Kyber.Arithmetic.barrett_pre (coefficient_normal_form +! error_2_.f_coefficients.[ i ] +! message.f_coefficients.[ i ]));
-          let result:Libcrux.Kem.Kyber.Arithmetic.wfPolynomialRingElement =
+                  i32) in
+          let resulti = cast_i32_b #3328 #(64*v v_K*3328) resulti in
+          let result =
             {
               result with
               Libcrux.Kem.Kyber.Arithmetic.f_coefficients
               =
               Rust_primitives.Hax.Monomorphized_update_at.update_at_usize result
                   .Libcrux.Kem.Kyber.Arithmetic.f_coefficients
-                i
-                (Libcrux.Kem.Kyber.Arithmetic.barrett_reduce ((coefficient_normal_form +!
+                i resulti
+            }
+          in
+          assert (inv result (i +! sz 1));
+          result)
+  in
+  admit(); //P-F
+  result
+#pop-options
+
+#push-options "--ifuel 0 --z3rlimit 100"
+let compute_ring_element_v v_K tt_as_ntt r_as_ntt error_2_ message =
+  let result:Libcrux.Kem.Kyber.Arithmetic.t_PolynomialRingElement_b (v v_K * 3328) =
+    Libcrux.Kem.Kyber.Arithmetic.cast_poly_b Libcrux.Kem.Kyber.Arithmetic.impl__PolynomialRingElement__ZERO
+  in
+  [@ inline_let]
+  let inv = fun (acc:t_PolynomialRingElement_b (v v_K * 3328)) (i:usize) ->
+    (v i <= 256) /\
+    (poly_range acc (v i * 3328)) in
+  let result:Libcrux.Kem.Kyber.Arithmetic.t_PolynomialRingElement_b (v v_K * 3328) =
+    Rust_primitives.Iterators.foldi_range #_ #_ #inv ({
+              Core.Ops.Range.f_start = sz 0;
+              Core.Ops.Range.f_end = v_K
+            }
+        <:
+        Core.Ops.Range.t_Range usize)
+      result
+      (fun result i ->
+          let product:Libcrux.Kem.Kyber.Arithmetic.wfPolynomialRingElement =
+            Libcrux.Kem.Kyber.Ntt.ntt_multiply (tt_as_ntt.[ i ]
+                <:
+                Libcrux.Kem.Kyber.Arithmetic.wfPolynomialRingElement)
+              (r_as_ntt.[ i ] <: Libcrux.Kem.Kyber.Arithmetic.wfPolynomialRingElement)
+          in
+          let result:t_PolynomialRingElement_b (v i * 3328) = 
+            down_cast_poly_b #(v v_K * 3328) #(v i * 3328) result in
+          let result:Libcrux.Kem.Kyber.Arithmetic.t_PolynomialRingElement_b ((v i + 1) * 3328) =
+            Libcrux.Kem.Kyber.Arithmetic.add_to_ring_element v_K result product
+          in
+          cast_poly_b result)
+  in
+  let result:Libcrux.Kem.Kyber.Arithmetic.t_PolynomialRingElement_b (64 * v v_K * 3328) =
+    Libcrux.Kem.Kyber.Ntt.invert_ntt_montgomery v_K result
+  in
+  [@ inline_let]
+  let inv = fun (acc:t_PolynomialRingElement_b (64 * v v_K * 3328)) (i:usize) -> 
+    (v i <= 256) /\
+    (forall (j:usize). (v j < v i) ==> i32_range ((acc <: t_PolynomialRingElement_b (64* v v_K * 3328)).f_coefficients.[j]) 3328) in
+  let result:Libcrux.Kem.Kyber.Arithmetic.t_PolynomialRingElement_b (64 * v v_K * 3328) =
+    Rust_primitives.Iterators.foldi_range #_ #_ #inv {
+              Core.Ops.Range.f_start = sz 0;
+              Core.Ops.Range.f_end = Libcrux.Kem.Kyber.Constants.v_COEFFICIENTS_IN_RING_ELEMENT
+            }
+      result 
+      (fun result i ->
+          let coefficient_normal_form: i32_b (nat_div_ceil (306921472*v v_K) 65536 + 1665) = 
+              Libcrux.Kem.Kyber.Arithmetic.montgomery_reduce 
+                           (Libcrux.Kem.Kyber.Arithmetic.mul_i32_b #(64 * v v_K * 3328) #1441
+                           result.Libcrux.Kem.Kyber.Arithmetic.f_coefficients.[ i ] 
+                           (1441l <: Libcrux.Kem.Kyber.Arithmetic.i32_b 1441)) in
+          let resulti : i32_b 3328 = 
+            (Libcrux.Kem.Kyber.Arithmetic.barrett_reduce ((coefficient_normal_form +!
                         (error_2_.Libcrux.Kem.Kyber.Arithmetic.f_coefficients.[ i ] <: i32)
                         <:
                         i32) +!
@@ -282,16 +266,25 @@ let compute_ring_element_v v_K tt_as_ntt r_as_ntt error_2_ message =
                       <:
                       i32)
                   <:
-                  i32)
+                  i32) in
+          let resulti = cast_i32_b #3328 #(64*v v_K*3328) resulti in
+          let result =
+            {
+              result with
+              Libcrux.Kem.Kyber.Arithmetic.f_coefficients
+              =
+              Rust_primitives.Hax.Monomorphized_update_at.update_at_usize result
+                  .Libcrux.Kem.Kyber.Arithmetic.f_coefficients
+                i resulti
             }
-            <:
-            Libcrux.Kem.Kyber.Arithmetic.wfPolynomialRingElement
           in
           result)
   in
   admit(); //P-F
   result
+#pop-options
 
+#push-options "--ifuel 0 --z3rlimit 100"
 let compute_vector_u
       (v_K: usize)
       (a_as_ntt: t_Array (t_Array Libcrux.Kem.Kyber.Arithmetic.wfPolynomialRingElement v_K) v_K)
@@ -301,119 +294,116 @@ let compute_vector_u
   in
   let acc_t = t_Array Libcrux.Kem.Kyber.Arithmetic.wfPolynomialRingElement v_K in
   [@ inline_let]
-  let inv = fun (acc:acc_t) (i:usize) -> True in
+  let inv0 = fun (acc:t_Array wfPolynomialRingElement v_K) (i:usize) -> 
+   (v i <= v v_K) /\
+   (forall (j k:usize). (v j >= v i /\ v j < v v_K /\ v k < 256) ==> v (((acc.[j] <: Libcrux.Kem.Kyber.Arithmetic.wfPolynomialRingElement).f_coefficients.[k]) <: i32) == 0)
+  in
   let result:t_Array Libcrux.Kem.Kyber.Arithmetic.wfPolynomialRingElement v_K =
-    Rust_primitives.Iterators.foldi_slice #(t_Array Libcrux.Kem.Kyber.Arithmetic.wfPolynomialRingElement v_K) #acc_t #inv
+    Rust_primitives.Iterators.foldi_slice #(t_Array Libcrux.Kem.Kyber.Arithmetic.wfPolynomialRingElement v_K) #acc_t #inv0
       a_as_ntt
       result
       (fun result temp_1_ ->
           let result:t_Array Libcrux.Kem.Kyber.Arithmetic.wfPolynomialRingElement v_K = result in
+          let orig_result = result in
+          let orig_result_cast = (cast_vector_b #v_K #3328 #(v v_K * 3328) orig_result) in
           let i, row:(usize & t_Array Libcrux.Kem.Kyber.Arithmetic.wfPolynomialRingElement v_K) =
             temp_1_
           in
           [@ inline_let]
-          let inv = fun (acc:acc_t) (i:usize) -> True in
-          let result:t_Array Libcrux.Kem.Kyber.Arithmetic.wfPolynomialRingElement v_K =
-            Rust_primitives.Iterators.foldi_slice #Libcrux.Kem.Kyber.Arithmetic.wfPolynomialRingElement #acc_t #inv
+          let inv1 = fun (acc:t_Array (Libcrux.Kem.Kyber.Arithmetic.t_PolynomialRingElement_b (v v_K * 3328)) v_K) (inner:usize) ->
+             (v inner <= v v_K) /\
+             (forall (j:usize). (v j < v i /\ v j < v v_K) ==> acc.[j] == orig_result_cast.[j]) /\
+             (forall (j:usize). (v j > v i /\ v j < v v_K) ==> acc.[j] == orig_result_cast.[j]) /\
+             (poly_range (acc.[i] <: Libcrux.Kem.Kyber.Arithmetic.t_PolynomialRingElement_b (v v_K * 3328)) (v inner * 3328))
+          in
+          assert (forall (k:usize). (v k < 256) ==> v (result.[i] <: wfPolynomialRingElement).f_coefficients.[k] == 0);
+          assert(inv1 orig_result_cast (sz 0));
+          let result:t_Array (Libcrux.Kem.Kyber.Arithmetic.t_PolynomialRingElement_b (v v_K * 3328)) v_K =
+            Rust_primitives.Iterators.foldi_slice #Libcrux.Kem.Kyber.Arithmetic.wfPolynomialRingElement #(t_Array (Libcrux.Kem.Kyber.Arithmetic.t_PolynomialRingElement_b (v v_K * 3328)) v_K) #inv1
               row
-              result
+              orig_result_cast
               (fun result temp_1_ ->
-                  let result:t_Array Libcrux.Kem.Kyber.Arithmetic.wfPolynomialRingElement v_K =
-                    result
-                  in
                   let j, a_element:(usize & Libcrux.Kem.Kyber.Arithmetic.wfPolynomialRingElement) =
                     temp_1_
                   in
-                  admit();
+                  let resulti = down_cast_poly_b #(v v_K * 3328) #(v j * 3328) result.[i] in
                   let product:Libcrux.Kem.Kyber.Arithmetic.wfPolynomialRingElement =
                     Libcrux.Kem.Kyber.Ntt.ntt_multiply a_element
                       (r_as_ntt.[ j ] <: Libcrux.Kem.Kyber.Arithmetic.wfPolynomialRingElement)
                   in
-                  admit(); //pre for add_to_ring
-                  let result:t_Array Libcrux.Kem.Kyber.Arithmetic.wfPolynomialRingElement v_K =
+                  let product_sum:Libcrux.Kem.Kyber.Arithmetic.t_PolynomialRingElement_b ((v j + 1) * 3328)  =
+                      (Libcrux.Kem.Kyber.Arithmetic.add_to_ring_element #(v j * 3328) #3328 v_K
+                          resulti
+                          product) in
+                  let product_sum:(Libcrux.Kem.Kyber.Arithmetic.t_PolynomialRingElement_b (v v_K * 3328)) = cast_poly_b #((v j+1)* 3328) #(v v_K * 3328) product_sum in 
+                  let result:t_Array (Libcrux.Kem.Kyber.Arithmetic.t_PolynomialRingElement_b (v v_K * 3328)) v_K =
                     Rust_primitives.Hax.Monomorphized_update_at.update_at_usize result
                       i
-                      (Libcrux.Kem.Kyber.Arithmetic.add_to_ring_element v_K
-                          (result.[ i ] <: Libcrux.Kem.Kyber.Arithmetic.wfPolynomialRingElement)
-                          product
-                        <:
-                        Libcrux.Kem.Kyber.Arithmetic.wfPolynomialRingElement)
+                      product_sum
                   in
                   result)
           in
-          admit();
-          let result:t_Array Libcrux.Kem.Kyber.Arithmetic.wfPolynomialRingElement v_K =
+          assert (forall (j:usize). (v j < v i /\ v j < v v_K) ==> result.[j] == orig_result_cast.[j]);
+          assert (forall (j:usize). (v j > v i /\ v j < v v_K) ==> result.[j] == orig_result_cast.[j]);
+          let result = cast_vector_b #v_K #(v v_K * 3328) #(64 * v v_K * 3328) result in
+          let orig_result_cast = (cast_vector_b #v_K #3328 #(64 * v v_K * 3328) orig_result) in
+          assert (forall (j:usize). (v j < v i /\ v j < v v_K) ==> result.[j] == orig_result_cast.[j]);
+          let resulti = result.[i] in
+          let result =
             Rust_primitives.Hax.Monomorphized_update_at.update_at_usize result
               i
-              (Libcrux.Kem.Kyber.Ntt.invert_ntt_montgomery v_K
-                  (result.[ i ] <: Libcrux.Kem.Kyber.Arithmetic.wfPolynomialRingElement)
-                <:
-                Libcrux.Kem.Kyber.Arithmetic.wfPolynomialRingElement)
+              (Libcrux.Kem.Kyber.Ntt.invert_ntt_montgomery v_K resulti)
+           in
+          [@ inline_let]
+          let inv2 = fun (acc:t_Array (Libcrux.Kem.Kyber.Arithmetic.t_PolynomialRingElement_b (64*v v_K * 3328)) v_K) (inner:usize) -> 
+             (v inner <= 256) /\
+             (forall (j:usize). (v j < v i /\ v j < v v_K) ==> acc.[j] == orig_result_cast.[j]) /\
+             (forall (j:usize). (v j > v i /\ v j < v v_K) ==> acc.[j] == orig_result_cast.[j]) /\
+             (forall (j:usize). (v j < v inner) ==> (i32_range (acc.[i] <: Libcrux.Kem.Kyber.Arithmetic.t_PolynomialRingElement_b (64*v v_K * 3328)).f_coefficients.[j] 3328))
+             // And all indexes above v inner are unchanged from result1
           in
-          Core.Iter.Traits.Iterator.f_fold (Core.Iter.Traits.Collect.f_into_iter ({
-                    Core.Ops.Range.f_start = sz 0;
-                    Core.Ops.Range.f_end
-                    =
-                    Libcrux.Kem.Kyber.Constants.v_COEFFICIENTS_IN_RING_ELEMENT
-                  }
-                  <:
-                  Core.Ops.Range.t_Range usize)
-              <:
-              Core.Ops.Range.t_Range usize)
+          assert (forall (j:usize). (v j < v i /\ v j < v v_K) ==> result.[j] == orig_result_cast.[j]);
+          assert (forall (j:usize). (v j > v i /\ v j < v v_K) ==> result.[j] == orig_result_cast.[j]);
+          assert (inv2 result (sz 0));
+          let result:t_Array (Libcrux.Kem.Kyber.Arithmetic.t_PolynomialRingElement_b (64*v v_K * 3328)) v_K =
+            Rust_primitives.Iterators.foldi_range #_ #(t_Array (Libcrux.Kem.Kyber.Arithmetic.t_PolynomialRingElement_b (64*v v_K * 3328)) v_K) #inv2 {
+              Core.Ops.Range.f_start = sz 0;
+              Core.Ops.Range.f_end = Libcrux.Kem.Kyber.Constants.v_COEFFICIENTS_IN_RING_ELEMENT
+            }
             result
             (fun result j ->
-                let result:t_Array Libcrux.Kem.Kyber.Arithmetic.wfPolynomialRingElement v_K =
-                  result
-                in
-                assume (range (v (result.[i]).(j) * 1441) i32_inttype);
-
-                let j:usize = j in
-                let coefficient_normal_form =
-                  Libcrux.Kem.Kyber.Arithmetic.montgomery_reduce (
-                  Libcrux.Kem.Kyber.Arithmetic.mul_i32_b
-                  ((result.[ i ]
-                          <:
-                          Libcrux.Kem.Kyber.Arithmetic.wfPolynomialRingElement)
-                          .Libcrux.Kem.Kyber.Arithmetic.f_coefficients.[ j ]
-                        <:
-                        Libcrux.Kem.Kyber.Arithmetic.i32_b 3328)
-                   (1441l <: Libcrux.Kem.Kyber.Arithmetic.i32_b 1441)) 
-                in
-                assume (range (v coefficient_normal_form + v (error_1_.[i]).( j )) i32_inttype);
-//                assume (Libcrux.Kem.Kyber.Arithmetic.barrett_pre (coefficient_normal_form +! (error_1_.[i]).( j ))); 
-                let result:t_Array Libcrux.Kem.Kyber.Arithmetic.wfPolynomialRingElement v_K =
+                let result: t_Array (Libcrux.Kem.Kyber.Arithmetic.t_PolynomialRingElement_b (64*v v_K * 3328)) v_K = result in
+                let resulti:(Libcrux.Kem.Kyber.Arithmetic.t_PolynomialRingElement_b (64*v v_K * 3328)) = result.[ i ]  <:  (Libcrux.Kem.Kyber.Arithmetic.t_PolynomialRingElement_b (64*v v_K * 3328)) in
+                let coefficient_normal_form: i32_b (nat_div_ceil (306921472*v v_K) 65536 + 1665) = 
+              Libcrux.Kem.Kyber.Arithmetic.montgomery_reduce 
+                           (Libcrux.Kem.Kyber.Arithmetic.mul_i32_b #(64 * v v_K * 3328) #1441
+                           resulti.(j) (1441l <: Libcrux.Kem.Kyber.Arithmetic.i32_b 1441)) in
+                let resultij: i32_b 3328 = (Libcrux.Kem.Kyber.Arithmetic.barrett_reduce 
+                                    (add_i32_b coefficient_normal_form ((error_1_.[ i ]
+                                    <:
+                                    Libcrux.Kem.Kyber.Arithmetic.wfPolynomialRingElement)
+                                    .Libcrux.Kem.Kyber.Arithmetic.f_coefficients.[ j ]))) in
+                let result =
                   Rust_primitives.Hax.Monomorphized_update_at.update_at_usize result
                     i
                     ({
                         (result.[ i ] <: Libcrux.Kem.Kyber.Arithmetic.wfPolynomialRingElement) with
                         Libcrux.Kem.Kyber.Arithmetic.f_coefficients
                         =
-                        Rust_primitives.Hax.Monomorphized_update_at.update_at_usize (result.[ i ]
-                            <:
-                            Libcrux.Kem.Kyber.Arithmetic.wfPolynomialRingElement)
-                            .Libcrux.Kem.Kyber.Arithmetic.f_coefficients
+                        Rust_primitives.Hax.Monomorphized_update_at.update_at_usize (resulti
+                            .Libcrux.Kem.Kyber.Arithmetic.f_coefficients)
                           j
-                          (Libcrux.Kem.Kyber.Arithmetic.barrett_reduce (coefficient_normal_form +!
-                                ((error_1_.[ i ]
-                                    <:
-                                    Libcrux.Kem.Kyber.Arithmetic.wfPolynomialRingElement)
-                                    .Libcrux.Kem.Kyber.Arithmetic.f_coefficients.[ j ]
-                                  <:
-                                  i32)
-                                <:
-                                i32)
-                            <:
-                            i32)
+                          resultij
                         <:
                         t_Array i32 (sz 256)
-                      }
-                      <:
-                      Libcrux.Kem.Kyber.Arithmetic.wfPolynomialRingElement)
-                in
-                result))
+                      }) in
+                result)
+        in
+        result)
   in
   admit(); //P-F
   result
+#pop-options
 
 let sample_matrix_A (v_K: usize) (seed: t_Array u8 (sz 34)) (transpose: bool) =
   let v_A_transpose:t_Array (t_Array Libcrux.Kem.Kyber.Arithmetic.wfPolynomialRingElement v_K) v_K =
